some tests worked

theories/L3_flattenedApp/test_wcbvEval.v
@@ -30,6 +30,37 @@ Definition mbt_main := main L1g_mbt. (* L1g main function *)
 Eval cbv in (wcbvEval 10 mbt_env mbt_main).
 
 
+(** vector addition **)
+Require Coq.Vectors.Vector.
+Print Fin.t.
+Print Vector.t.
+
+Definition vplus (n:nat) :
+  Vector.t nat n -> Vector.t nat n -> Vector.t nat n := (Vector.map2 plus).
+Definition v01 : Vector.t nat 2 :=
+  (Vector.cons nat 0 1 (Vector.cons nat 1 0 (Vector.nil nat))).
+Definition v23 : Vector.t nat 2 :=
+  (Vector.cons nat 2 1 (Vector.cons nat 3 0 (Vector.nil nat))).
+Definition vplus0123 := (vplus _ v01 v23).
+Quote Recursively Definition cbv_vplus0123 := (* [program] of Coq's answer *)
+  ltac:(let t:=(eval cbv in (vplus0123)) in exact t).
+Print cbv_vplus0123.
+(* [Term] of Coq's answer *)
+Definition ans_vplus0123 := Eval cbv in (main (program_Program cbv_vplus0123)).
+(* [program] of the program *)
+Quote Recursively Definition p_vplus0123 := vplus0123.
+Print p_vplus0123.
+Definition P_vplus0123 := Eval cbv in (program_Program p_vplus0123).
+Print P_vplus0123.
+Goal
+  let env := (env P_vplus0123) in
+  let main := (main P_vplus0123) in
+  wcbvEval 100 (env) (main) = Some ans_vplus0123.
+  vm_compute. reflexivity.
+Qed.
+
+
+
 Inductive List (A:Set) :=
   Nil: List A | Cons: forall (a:A) (bs:List A), List A.
 Definition tl (A:Set) (ls:List A) : List A :=
@@ -41,6 +72,39 @@ Print p_tl.
 Require Coq.Vectors.Vector.
 Print Fin.t.
 Print Vector.t.
+
+Definition vplus (n:nat) :
+  Vector.t nat n -> Vector.t nat n -> Vector.t nat n :=
+  Eval cbv in (Vector.map2 plus).
+Definition v01 : Vector.t nat 2 :=
+  (Vector.cons nat 0 1 (Vector.cons nat 1 0 (Vector.nil nat))).
+Definition v23 : Vector.t nat 2 :=
+  (Vector.cons nat 2 1 (Vector.cons nat 3 0 (Vector.nil nat))).
+Definition vplus0123 := (@vplus 2 v01 v23).
+Definition cbv_vplus0123 := Eval cbv in vplus0123.  (* evaluated by Coq *)
+Print cbv_vplus0123.
+(* program of Coq's result *)
+Quote Recursively Definition p_vplus0123 := (@vplus 2 v01 v23).
+Print p_vplus0123.
+Quote Definition q_vplus0123 := Eval cbv in (@vplus 2 v01 v23).
+Print q_vplus0123.
+Definition pP := Eval cbv in program_Program p_vplus0123.
+Print pP.
+(**
+Definition cbv_q_vplus0123 := Eval cbv in (term_Term (env pP) q_vplus0123).
+Print cbv_q_vplus0123.
+**)
+Definition cbv_env_pP := Eval cbv in (env pP).
+Print cbv_env_pP.
+Definition cbv_main_pP := Eval cbv in (main pP).
+Print cbv_main_pP.
+Eval cbv in (wcbvEval 100 cbv_env_pP cbv_main_pP).
+Goal
+  wcbvEval (env pP) 1000 (main pP) = Ret cbv_q_vplus0123.
+  vm_compute. reflexivity.
+Qed.
+
+
 
 Definition vplus (n:nat) :
   Vector.t nat n -> Vector.t nat n -> Vector.t nat n :=
